Juvix/Core/Main/Language/Value.lean
@@ -12,4 +12,45 @@ inductive Value : Type where
 
 abbrev Env : Type := List Value
 
+mutual
+  @[simp]
+  def Value.dom : (v : Value) → Set Name
+    | Value.unit => ∅
+    | Value.const _ => ∅
+    | Value.constr_app _ args_rev => Value.List.dom args_rev
+    | Value.closure env body => Value.List.dom env ∪ body.dom
+
+  @[simp]
+  def Value.List.dom : (vs : List Value) → Set Name
+    | [] => ∅
+    | v :: vs => v.dom ∪ Value.List.dom vs
+end
+
+@[simp]
+def Env.dom : (env : Env) → Set Name :=
+  Value.List.dom
+
+lemma Value.dom_env (v : Value) (env : Env) : v ∈ env → v.dom ⊆ env.dom := by
+  intro h
+  induction env generalizing v
+  case nil =>
+    contradiction
+  case cons hd tl ih =>
+    cases h
+    case head =>
+      simp [Value.dom, Value.List.dom]
+    case tail hm =>
+      simp [Value.dom, Value.List.dom]
+      exact Set.subset_union_of_subset_right (ih v hm) hd.dom
+
+lemma Value.List.dom_append (vs₁ vs₂ : List Value) :
+  Value.List.dom (vs₁ ++ vs₂) = Value.List.dom vs₁ ∪ Value.List.dom vs₂ := by
+  induction vs₁ generalizing vs₂
+  case nil =>
+    simp [Value.List.dom]
+  case cons hd tl ih =>
+    simp [Value.List.dom]
+    rw [ih]
+    rw [Set.union_assoc]
+
 end Juvix.Core.Main
